which looks more intimidating. This inequality is attributed to the mathematician Augustin-Louis Cauchy; Hermann Schwarz gave the derivation given below.

The Cauchy-Schwarz inequality can be shown as follows. The inequality clearly holds if \(a=0\) or \(b=0\) (in this case, both sides of the inequality are zero). So we suppose now that \(a\neq 0\), \(b\neq 0\), and define \(\alpha=\|a\|\), \(\beta=\|b\|\). We observe that

\[0 \leq \|\beta a-\alpha b\|^{2}\] \[= \|\beta a\|^{2}-2(\beta a)^{T}(\alpha b)+\|\alpha b\|^{2}\] \[= \beta^{2}\|a\|^{2}-2\beta\alpha(a^{T}b)+\alpha^ 