

4. Apply elimination to produce the factors $L$ and $U$ for
$$
A=\left[\begin{array}{ll}
2 & 1 \\
8 & 7
\end{array}\right] \quad \text { and } \quad A=\left[\begin{array}{lll}
3 & 1 & 1 \\
1 & 3 & 1 \\
1 & 1 & 3
\end{array}\right] \text { and } A=\left[\begin{array}{lll}
1 & 1 & 1 \\
1 & 4 & 4 \\
1 & 4 & 8
\end{array}\right] .
$$
5. Factor $A$ into $L U$, and write down the upper triangular system $U x=c$ which appears after elimination, for
$$
A x=\left[\begin{array}{lll}
2 & 3 & 3 \\
0 & 5 & 7 \\
6 & 9 & 8
\end{array}\right]\left[\begin{array}{l}
u \\
v \\
w
\end{array}\right]=\left[\begin{array}{l}
2 \\
2 \\
5
\end{array}\right] .
$$
6. Find $E^2$ and $E^8$ and $E^{-1}$ if
$$
E=\left[\begin{array}{ll}
1 & 0 \\
6 & 1
\end{array}\right] .
$$
7. Find the products $F G H$ and $H G F$ if (with upper triangular zeros omitted)
$$
F=\left[\begin{array}{llll}
1 & & & \\
2 & 1 & & \\
0 & 0 & 1 & \\
0 & 0 & 0 & 1
\end{array}\right] \quad G=\left[\begin{array}{llll}
1 & & & \\
0 & 1 & & \\
0 & 2 & 1 & \\
0 & 0 & 0 & 1
\end{array}\right] \quad H=\left[\begin{array}{llll}
1 & & & \\
0 & 1 & & \\
0 & 0 & 1 & \\
0 & 0 & 2 & 1
\end{array}\right] .
$$
8. (Second proof of $A=L U$ ) The third row of $U$ comes from the third row of $A$ by subtracting multiples of rows 1 and 2 (of $U!$ ):
$$
\text { row } \left.3 \text { of } U=\text { row } 3 \text { of } A-\ell_{31}(\text { row } 1 \text { of } U)-\ell_{32} \text { (row } 2 \text { of } U\right) \text {. }
$$
(a) Why are rows of $U$ subtracted off and not rows of $A$ ? Answer: Because by the time a pivot row is used, . $\qquad$
(b) The equation above is the same as
$$
\text { row } 3 \text { of } A=\ell_{31}(\text { row } 1 \text { of } U)+\ell_{32}(\text { row } 2 \text { of } U)+1(\text { row } 3 \text { of } U) \text {. }
$$

Which rule for matrix multiplication makes this row 3 of $L$ times $U$ ?
The other rows of $L U$ agree similarly with the rows of $A$.
9. (a) Under what conditions is the following product nonsingular?
$$
A=\left[\begin{array}{ccc}
1 & 0 & 0 \\
-1 & 1 & 0 \\
0 & -1 & 1
\end{array}\right]\left[\begin{array}{lll}
d_1 & & \\
& d_2 & \\
& & d_3
\end{array}\right]\left[\begin{array}{ccc}
1 & -1 & 0 \\
0 & 1 & -1 \\
0 & 0 & 1
\end{array}\right] .
$$
(b) Solve the system $A x=b$ starting with $L c=b$ :
$$
\left[\begin{array}{ccc}
1 & 0 & 0 \\
-1 & 1 & 0 \\
0 & -1 & 1
\end{array}\right]\left[\begin{array}{l}
c_1 \\
c_2 \\
c_3
\end{array}\right]=\left[\begin{array}{l}
0 \\
0 \\
1
\end{array}\right]=b
$$
