\[\text{(a)}\quad b=\begin{bmatrix}1\\ 2\\ 2\end{bmatrix}\quad\text{and}\quad a=\begin{bmatrix}1\\ 1\\ 1\end{bmatrix}.\qquad\quad\text{(b)}\quad b=\begin{bmatrix}1\\ 3\\ 1\end{bmatrix}\quad\text{and}\quad a=\begin{bmatrix}-1\\ -3\\ -1\end{bmatrix}.\]

**18.**: _Draw_ the projection of \(b\) onto \(a\) and also compute it from \(p=\widehat{xa}\):

\[\text{(a)}\quad b=\begin{bmatrix}\cos\theta\\ \sin\theta\end{bmatrix}\quad\text{and}\quad a=\begin{bmatrix}1\\ 0\end{bmatrix}.\qquad\quad\text{(b)}\quad b=\begin{bmatrix}1\\ 1\end{bmatrix}\quad\text{and}\quad a=\begin{bmatrix}1\\ -1\end{bmatrix}.\]
**19.**: In Problem 17, find the projection matrix \(P=aa^{\mathrm{T}}/a^{\mathrm{T}}a\) onto the line through each vector \(a\). Verify in both cases that \(P^{2}=P\). Multiply \(Pb\) in each case to compute the projection \(p\).
**20.**: Construct the projection matrices \(P_{1}\) and \(P_{2}\) onto the lines through the \(a\)'s in Problem 18. Is it true that \((P_{1}+P_{2})^{2}=P_{1}+P_{2}\)? This _would_ be true if \(P_{1}P_{2}=0\).
**For Problems 21-26, consult the accompanying figures.**

**21.**: Compute the projection matrices \(aa^{\mathrm{T}}/a^{\mathrm{T}}a\) onto the lines through \(a_{1}=(-1,2,2)\) and \(a_{2}=(2,2,-1)\), Multiply those projection matrices and explain why their product \(P_{1}P_{2}\) is what it is.
**22.**: Project \(b=(1,0,0)\) onto the lines through \(a_{1}\) and \(a_{2}\) in Problem 21 and also onto \(a_{3}=(2,-1,2)\). Add the three projections \(p_{1}+p_{2}+p_{3}\).
**23.**: Continuing Problems 21-22, find the projection matrix \(P_{3}\) onto \(a_{3}=(2,-1,2)\). Verify that \(P_{1}+P_{2}+P_{3}=I\). The basis \(a_{1}\), \(a_{2}\), \(a_{3}\) is orthogonal!
**24.**: Project the vector \(b=(1,1)\) onto the lines through \(a_{1}=(1,0)\) and \(a_{2}=(1,2)\). Draw the projections \(p_{1}\) and \(p_{2}\) and add \(p_{1}+p_{2}\). The projections do not add to \(b\) because the \(a\)'s are not orthogonal.
**25.**: In Problem 24, the projection of \(b\) onto the _plane_ of \(a_{1}\) and \(a_{2}\) will equal \(b\). Find \(P=A(A^{\mathrm{T}}A)^{-1}A^{\mathrm{T}}\) for \(A=[a_{1}\ \ a_{2}]\begin{bmatrix}1\ 1\\ 0\ 2\end{bmatrix}\).

 