

**21.**: Best line is \(\begin{bmatrix}a_{1}^{\mathsf{T}}a_{1}&-a_{1}^{\mathsf{T}}a_{2}\\ -a_{1}^{\mathsf{T}}a_{2}&a_{2}^{\mathsf{T}}a_{2}\end{bmatrix}\begin{bmatrix} \widehat{x}_{1}\\ \widehat{x}_{2}\end{bmatrix}=\begin{bmatrix}a_{1}^{\mathsf{T}}b\\ -a_{2}^{\mathsf{T}}b\end{bmatrix}\); \(\widehat{x}=\begin{bmatrix}2\\ 1\end{bmatrix}\).
**23.**: \(C=(A^{\mathsf{T}}A)^{-1}A^{\mathsf{T}}b\), \(A^{\mathsf{T}}=[1\cdots 1]\), \(b=(y_{1},\,\ldots,\,y_{m})^{\mathsf{T}}\) then

\(C=\frac{A^{\mathsf{T}}b}{A^{\mathsf{T}}A}=\frac{y_{1}+\cdots+y_{m}}{m}\).
**25.**: \(A=\begin{smallmatrix}1&-1&1\\ 1&0&0\\ 1&1&1\\ 1&2&4\end{smallmatrix}\); \(x=\begin{bmatrix}C\\ D\\ E\end{bmatrix}\); \(b=\begin{bmatrix}2\\ 0\\ -3\\ -5\end{bmatrix}\).
**27.**: (a) \(a^{\mathsf{T}}a=m\), \(a^{\mathsf{T}}b=b_{1}+\cdots+b_{m}\). Therefore \(\widehat{x}\) is the mean of the \(b\)'s. (b) The variance is \(\|e\|^{2}=\sum_{i=1}^{m}(b_{i}-\widehat{x})^{2}\). (c) \(p=(3,3,3)\), \(e=(-2,-1,3)\), \(p^{\mathsf{T}}e=0\). \(P=\frac{1}{3}\begin{bmatrix}1&1&1\\ 1&1&1\\ 1&1&1\end{bmatrix}\).
**29.**: \((\widehat{x}-x)(\widehat{x}-x)^{\mathsf{T}}=(A^{\mathsf{T}}A)^{-1}A^{\mathsf{ T}}[(b-Ax)(b-Ax)^{\mathsf{T}}]A(A^{\mathsf{T}}A)^{-1}\). For independent errors, substituting \((b-Ax)(b-Ax)^{\mathsf{T}}=\sigma^{2}I\) gives the _covariance matrix_\((A^{\mathsf{T}}A)^{-1}A^{\mathsf{T}}\sigma^{2}A(A^{\mathsf{T}}A)^{-1}\). This simplifies to \(\sigma^{2}(A^{\mathsf{T}}A)^{-1}\): neat formula for the covariance matrix.
**31.**: \(\frac{1}{10}b_{10}+\frac{9}{10}\widehat{x}_{9}=\frac{1}{10}(b_{1}+\cdots+b_{1 0})\).
**33.**: \(\begin{bmatrix}1&0\\ 1&1\\ 1&3\\ 1&4\end{bmatrix}\begin{bmatrix}C\\ D\end{bmatrix}=\begin{bmatrix}8\\ 8\\ 20\end{bmatrix}\). Change right side to \(p=\begin{bmatrix}1\\ 5\\ 13\\ 17\end{bmatrix}\); \(\widehat{x}=\begin{bmatrix}1\\ 4\end{bmatrix}\) solves \(A\widehat{x}=p\).
**35.**: Closest parabola: \(\begin{bmatrix}1&0&0\\ 1&1&1\\ 1&3&9\\ 1&4&16\end{bmatrix}\begin{bmatrix}C\\ D\end{bmatrix}=\begin{bmatrix}0\\ 8\\ 8\\ 20\end{bmatrix}\).

\(A^{\mathsf{T}}A\widehat{x}=\begin{bmatrix}4&8&26\\ 8&26&92\\ 26&92&338\end{bmatrix}\begin{bmatrix}\widehat{C}\\ \widehat{D}\\ \widehat{E}\end{bmatrix}=\begin{bmatrix}36\\ 112\\ 400\end{bmatrix}\).
**37.**: (a) The best line is \(x=1+4t\), which goes through the center point \((\widehat{t},\,\widehat{b})=(2,\,9)\). (b) From the first equation: \(Cm+D\sum t_{i}=\sum b_{i}\). Divide by \(m\) to get \(C+D\widehat{t}=\widehat{b}\).
**39.**: \(\widehat{x}_{W}=\frac{w_{1}^{2}b_{1}+\cdots+w_{m}^{2}b_{m}}{w_{1}^{2}+\cdots+w_ {m}^{2}}\).
**41.**: \(\widehat{x}_{W}=(1/21,4/7)\); \(A\widehat{x}_{W}=(1/21,13/21,25/21)\),

\(b-A\widehat{x}_{W}=(-1/21,8/21,-4/2