(c) The vectors \(\alpha_{1}^{\prime}\), \(\alpha_{2}^{\prime}\), \(\alpha_{3}^{\prime}\) are all of the form \((y_{1}\), \(y_{2}\), \(y_{3}\), \(y_{4})\) with \(y_{3}=2y_{1}\) and thus they are in \(W\). One can see at a glance that they are independent. (d) The matrix \(P\) has for its columns \[P_{j}=[\alpha_{j}^{\prime}]_{\emptyset}\] where \(\emptyset=\{\alpha_{1},\,\alpha_{2},\,\alpha_{3}\}\). The equations (2-26) tell us how to find the coordinate matrices for \(\alpha_{1}^{\prime}\), \(\alpha_{2}^{\prime}\), \(\alpha_{3}^{\prime}\). For example with \(\beta=\alpha_{1}^{\prime}\) we have \(b_{1}=1\), \(b_{2}=0\), \(b_{3}=2\), \(b_{4}=0\), and \[\begin{array}{r@{\quad}l@{\quad}l}x_{1}=\quad&1-\frac{1}{3}(0)\,+\frac{2}{3}( 0)\,=\quad&1\\ x_{2}=\quad&-1\,+\frac{5}{6}(0)\,-\frac{2}{3}(0)\,=\,-1\\ x_{3}=\quad&-\frac{1}{6}(0)\,+\frac{1}{3}(0)\,=\quad&0.\end{array}\] Thus \(\alpha_{1}^{\prime}=\alpha_{1}-\alpha_{2}\). Similarly we obtain \(\alpha_{2}^{\prime}=\alpha_{2}\) and \(\alpha_{3}^{\prime}=2\alpha_{1}-\,2\alpha_{2}+\alpha_{3}\). Hence \[P=\!\left[\begin{array}{ccc}1\quad&0\quad&2\\ -1\quad&1\quad&-2\\ 0\quad&0\quad&1\end{array}\right]\] Now let us see how we would answer the questions by the second method which we described. We form the \(4\times 3\) matrix \(B\) with column vectors \(\alpha_{1}\), \(\alpha_{2}\), \(\alpha_{3}\): \[B=\begin{bmatrix}1&0&-2\\ 2&2&0\\ 2&0&-4\\ 1&1\quad&3\end{bmatrix}\] We inquire for which \(y_{1}\), \(y_{2}\), \(y_{3}\), \(y_{4}\) the system \(BX=Y\) has a solution. \[\begin{bmatrix}1&0&-2\quad&y_{1}\\ 2&2\quad&0\quad&y_{2}\\ 2&0\quad&-4\quad&y_{3}\\ 1&1\quad&3\quad&y_{4}\end{bmatrix}\!\!\longrightarrow\!\!\begin{bmatrix}1 \quad&0\quad&-2\quad&y_{1}\\ 0\quad&2\quad&4\quad&y_{2}-2y_{1}\\ 0\quad&0\quad&0\quad&y_{3}-2y_{1}\\ 0\quad&1\quad&5\quad&y_{4}-y_{1}\end{bmatrix}\!\!\longrightarrow\!\!\! \begin{bmatrix}1\quad&0\quad&-2\quad&y_{1}\\ 0\quad&2\quad&4\quad&y_{2}-2y_{1}\\ 0\quad&0\quad&0\quad&y_{3}-2y_{1}\\ 0\quad&1\quad&5\quad&y_{4}-y_{1}\end{bmatrix}\!\!\longrightarrow\!\!\! \begin{bmatrix}0\quad&0\quad&y_{1}-\frac{1}{3}y_{2}+\frac{2}{3}y_{4}\\ 0\quad&0\quad&1\quad&\frac{1}{6}(2y_{4}-y_{2})\\ 0\quad&1\quad&0\quad&-y_{1}+\frac{8}{6}y_{2}-\frac{2}{3}y_{4}\\ 0\quad&0\quad&y_{3}-2y_{1}\end{bmatrix}\!\!\longrightarrow\!\!\!\begin{bmatrix} 1\quad&0\quad&y_{1}-\frac{1}{3}y_{2}+\frac{2}{3}y_{4}\\ 0\quad&0\quad&1\quad&\frac{1}{6}(2y_{4}-y_{2})\\ 0\quad&1\quad&0\quad&-y_{1}+\frac{8}{6}y_{2}-\frac{2}{3}y_{4}\\ 0\quad&0\quad&y_{3}-2y_{1}\end{bmatrix}\! 